src/program_proof/twophase/wrapper_proof.v
@@ -1,5 +1,5 @@
 From Perennial.goose_lang Require Import lang notation typing.
-From Perennial.goose_lang.lib Require Import map.impl list.impl list_slice.
+From Perennial.goose_lang.lib Require Import map.impl list.impl list.list_slice.
 From Perennial.goose_lang.ffi Require Import jrnl_ffi.
 From Perennial.goose_lang.ffi Require Import disk.
 From Goose.github_com.mit_pdos.goose_nfsd Require Import txn twophase.
@@ -21,6 +21,7 @@ Section proof.
   Existing Instances jrnl_spec_ext jrnl_spec_ffi_model jrnl_spec_ext_semantics jrnl_spec_ffi_interp
            jrnl_spec_interp_adequacy.
   Context `{!refinement_heapG Σ}.
+  Context `{!jrnlG Σ}.
 
   Implicit Types (N: namespace).
 
@@ -29,144 +30,262 @@ Section proof.
 
   Definition val_of_obj (o : obj) := val_of_list ((λ u, LitV (LitByte u)) <$> o).
 
-  Parameter ex_mapsto : addr → object → iProp Σ.
+  Definition jrnl_mapsto_own addr obj : iProp Σ :=
+    ∃ obj', jrnl_mapsto addr 1 obj' ∗ ⌜data_has_obj obj' addr obj⌝.
 
-  (* XXX: seems like objs_spec should really be switched to a gmap in twophase_linv_flat ? *)
-  Definition is_twophase_pre N l (γ γ' : buftxn_names) dinit objs_dom : iProp Σ :=
-    ∃ (txnl locksl : loc) ghs objs_spec,
-      let objs_dom_blknos := get_addr_set_blknos objs_dom in
-      "Histwophase_txnl" ∷ readonly (l ↦[TwoPhasePre.S :: "txn"] #txnl) ∗
-      "Histwophase_locksl" ∷ readonly (l ↦[TwoPhasePre.S :: "locks"] #locksl) ∗
-      "#Histxn_system" ∷ is_txn_system N γ ∗
+  Definition jrnl_maps_have_mt_changed (σj1 σj2: jrnl_map) (mt_changed: gmap addr versioned_object) :=
+    dom (gset addr) (jrnlData σj1) = dom (gset addr) (jrnlData σj2) ∧
+    map_Forall (λ addr vobj,
+      match mt_changed !! addr with
+      | Some vobj' =>
+        data_has_obj vobj.1 addr (committed vobj') ∧
+        data_has_obj vobj.2 addr (modified vobj')
+      | None => vobj.1 = vobj.2
+      end
+    ) (map_zip (jrnlData σj1) (jrnlData σj2)).
+
+  Definition is_twophase_pre l (γ γ' : buftxn_names Σ) dinit (objs_dom: gset addr) : iProp Σ :=
+    ∃ (txnl locksl : loc) ghs,
+      "#Hpre.txn" ∷ readonly (l ↦[TwoPhasePre.S :: "txn"] #txnl) ∗
+      "#Hpre.locks" ∷ readonly (l ↦[TwoPhasePre.S :: "locks"] #locksl) ∗
+      "#Histxn_system" ∷ is_txn_system Nbuftxn γ ∗
       "#Histxn" ∷ is_txn txnl γ.(buftxn_txn_names) dinit ∗
-      "#HlockMap" ∷ is_lockMap locksl ghs
-      (set_map addr2flat (dom (gset addr) objs_spec))
-      (twophase_linv_flat 0 ex_mapsto objs_spec γ).
+      "#HlockMap" ∷ is_lockMap locksl ghs (set_map addr2flat objs_dom)
+        (twophase_linv_flat 0 jrnl_mapsto_own γ) ∗
+      "#Htxn_cinv" ∷ txn_cinv Nbuftxn γ γ' ∗
+      "%Hvalids" ∷ ⌜set_Forall valid_addr objs_dom⌝.
 
-  Definition is_twophase_started N l γ γ' dinit objs_dom j K e1 e2 : iProp Σ :=
-    ∃ (txnl locksl : loc) ls ghs σj1 σj2 objs_spec,
-    let objs_dom_blknos := get_addr_set_blknos objs_dom in
-    "Htwophase.txn" ∷ readonly (l ↦[TwoPhase.S :: "txn"] #txnl) ∗
-    "Htwophase.locks" ∷ readonly (l ↦[TwoPhase.S :: "locks"] #locksl) ∗
-    "%Halways_steps" ∷ ⌜ always_steps e1 σj1 e2 σj2 ⌝ ∗
-    "#Histxn_system" ∷ is_txn_system N γ ∗
-    "#Histxn" ∷ is_txn txnl γ.(buftxn_txn_names) dinit ∗
-    "#HlockMap" ∷ is_lockMap locksl ghs
-      (set_map addr2flat (dom (gset addr) objs_spec))
-      (twophase_linv_flat 0 ex_mapsto objs_spec γ) ∗
-    "#Htxn_cinv" ∷ txn_cinv N γ γ' ∗
-    "#Hspec_ctx" ∷ spec_ctx ∗
-    "Hj" ∷ j ⤇ K (Atomically ls e1) ∗
-    (* TODO: this should be at least all the na_crash_invs in σj1 and the ephemeral values
-       for σj2 *)
-    "Hlock_resources" ∷ True.
+  Definition is_twophase_started l γ dinit objs_dom j K ls e1 e2 : iProp Σ :=
+    ∃ σj1 σj2 mt_changed,
+      (* mark: do we need is_twophase_pre in here too? *)
+      "Hj" ∷ j ⤇ K (Atomically ls e1) ∗
+      "Htwophase" ∷ is_twophase_raw
+        l γ dinit 0 jrnl_mapsto_own objs_dom mt_changed ∗
+      "%Halways_steps" ∷ ⌜ always_steps e1 σj1 e2 σj2 ⌝ ∗
+      "%Hmt_changed" ∷ ⌜ jrnl_maps_have_mt_changed σj1 σj2 mt_changed ⌝.
 
-  Definition is_twophase_releasable N l γ γ' dinit objs_dom : iProp Σ :=
-    ∃ (txnl locksl : loc) ghs (σj : gmap addr obj) objs_spec,
-    let objs_dom_blknos := get_addr_set_blknos objs_dom in
-    "Htwophase.txn" ∷ readonly (l ↦[TwoPhase.S :: "txn"] #txnl) ∗
-    "Htwophase.locks" ∷ readonly (l ↦[TwoPhase.S :: "locks"] #locksl) ∗
-    "#Histxn_system" ∷ is_txn_system N γ ∗
-    "#Histxn" ∷ is_txn txnl γ.(buftxn_txn_names) dinit ∗
-    "#HlockMap" ∷ is_lockMap locksl ghs
-      (set_map addr2flat (dom (gset addr) objs_spec))
-      (twophase_linv_flat 0 ex_mapsto objs_spec γ) ∗
-    "#Htxn_cinv" ∷ txn_cinv N γ γ' ∗
-    (* TODO: this should be at least all the na_crash_invs in σj1 and the ephemeral values
-       for σj *)
-    "Hlock_resources" ∷ True.
+  Definition is_twophase_releasable l γ (objs_dom: gset addr) : iProp Σ :=
+    ∃ locks_held mt_changed σj1 σj2,
+      (* mark: do we need is_twophase_pre in here too? *)
+      "Hlocks" ∷ is_twophase_locks
+        l γ 0 jrnl_mapsto_own (set_map addr2flat objs_dom) locks_held ∗
+      "Hlinvs" ∷ ([∗ list] flat_a ∈ locks_held, (
+        "Hlinv" ∷ twophase_linv_flat 0 jrnl_mapsto_own γ flat_a
+      )) ∗
+      "%Hlocks_held" ∷ ⌜
+        set_map addr2flat (dom (gset addr) mt_changed) =
+        (list_to_set locks_held: gset u64)
+      ⌝ ∗
+      "%Hmt_changed" ∷ ⌜ jrnl_maps_have_mt_changed σj1 σj2 mt_changed ⌝ ∗
+      "%Hvalids" ∷ ⌜set_Forall valid_addr objs_dom⌝.
 
-  Theorem wpc_Init' N (d: loc) γ dinit logm objs_dom k :
-    {{{ is_txn_durable γ dinit logm }}}
-      TwoPhase__Init' #d @ k; ⊤
-    {{{ γ' (l: loc), RET #l; is_twophase_pre N l γ γ' dinit objs_dom}}}
-    {{{ ∃ γ' logm', ⌜ γ'.(buftxn_txn_names).(txn_kinds) = γ.(buftxn_txn_names).(txn_kinds) ⌝ ∗
-        is_txn_durable γ' dinit logm' ∗
-       (⌜ γ' = γ ⌝ ∨ txn_cinv N γ γ') }}}.
-  Proof. Admitted.
+  Theorem wpc_Init N (d: loc) γ dinit logm mt k :
+    N ## invN →
+    N ## invariant.walN →
+    map_Forall (mapsto_valid γ) mt →
+    {{{
+      "Htxn_durable" ∷ is_txn_durable γ dinit logm ∗
+      "Hmapstos" ∷ ([∗ map] a ↦ obj ∈ mt,
+        "Hdurable_mapsto" ∷ durable_mapsto_own γ a obj ∗
+        "Hjrnl_mapsto" ∷ jrnl_mapsto_own a obj
+      )
+    }}}
+      Init #d @ k; ⊤
+    {{{
+      γ' (l: loc), RET #l;
+      "Htwophase" ∷ is_twophase_pre
+        l γ γ' dinit (dom (gset addr) mt)
+    }}}
+    {{{ ∃ γ' logm',
+      is_txn_durable γ' dinit logm' ∗
+      (⌜ γ' = γ ⌝ ∨ txn_cinv Nbuftxn γ γ')
+    }}}.
+  Proof.
+    iIntros (HinvN HwalN Hvalids Φ Φc) "(?&?) HΦ".
+    iNamed.
+    wpc_call.
+    {
+      iExists _, _.
+      iFrame.
+      auto.
+    }
+    wpc_apply (wpc_MkTxn Nbuftxn with "Htxn_durable").
+    1-2: solve_ndisj.
+    iSplit.
+    {
+      iDestruct "HΦ" as "[HΦ _]".
+      iFrame.
+    }
+    iModIntro.
+    iIntros (? txnl) "
+      (#Histxn&#Histxn_system&Htxn_cancel&#Htxn_cinv&%Htxn_kinds)
+    ".
+    iApply wpc_cfupd.
+    iCache with "HΦ Htxn_cancel".
+    {
+      iDestruct "HΦ" as "[HΦ _]".
+      iModIntro.
+      iMod "Htxn_cancel"; first by lia.
+      iMod "Htxn_cancel".
+      iDestruct "Htxn_cancel" as (?) "Htxn_cancel".
+      iModIntro.
+      iApply "HΦ".
+      iExists _, _.
+      iFrame "∗ #".
+      auto.
+    }
+    wpc_frame.
+    iMod (twophase_init_locks with "Histxn_system Hmapstos") as "?".
+    1-2: set_solver.
+    {
+      intros a Hin.
+      apply elem_of_dom in Hin.
+      destruct Hin as [obj Hacc].
+      apply Hvalids in Hacc.
+      destruct Hacc as (Hvalid&_&_).
+      assumption.
+    }
+    iNamed.
+    wp_apply (
+      wp_MkLockMap _ (twophase_linv_flat 0 jrnl_mapsto_own γ)
+      with "[Hlinvs]"
+    ).
+    {
+      iApply (big_sepS_impl with "Hlinvs").
+      iIntros (addr_flat) "!> %Hin $".
+    }
+    iIntros (locksl ?) "#Hlocks".
+    wp_apply wp_allocStruct; first by auto.
+    iIntros (prel) "Hprel".
+    iDestruct (struct_fields_split with "Hprel") as "(?&?&_)".
+    iNamed.
+    iMod (readonly_alloc_1 with "txn") as "#Hpre.txn".
+    iMod (readonly_alloc_1 with "locks") as "#Hpre.locks".
+    wp_pures.
+    iIntros "[? ?]".
+    iNamed.
 
-  Theorem wp_TwoPhase__Begin' N l ls γ γ' dinit objs_dom j K e1 :
-    {{{ is_twophase_pre N l γ γ' dinit objs_dom ∗
-        j ⤇ K (Atomically ls e1) }}}
-      TwoPhase__Begin' #l
-    {{{ tph, RET #tph;
-        is_twophase_started N tph γ γ' dinit objs_dom
-                            j K e1 e1 }}}.
-  Proof. Admitted.
+    iApply "HΦ".
+    iExists _, _, _.
+    iFrame (Htxn_kinds) "#".
+    iPureIntro.
+    intros addr Hin.
+    apply elem_of_dom in Hin.
+    destruct Hin as [obj Hacc].
+    apply Hvalids in Hacc.
+    destruct Hacc as (Hvalid&_&_).
+    assumption.
+  Qed.
 
-  Theorem wp_TwoPhase__CommitNoRelease' N l γ γ' dinit objs_dom j K e1 v :
-    {{{ is_twophase_started N l γ γ' dinit objs_dom j K e1 (SOMEV v) }}}
+  Theorem wp_TwoPhase__Begin' N prel ls γ γ' dinit objs_dom j K e1 :
+    {{{
+      "Htwophase" ∷ is_twophase_pre prel γ γ' dinit objs_dom ∗
+      "Hatom" ∷ j ⤇ K (Atomically ls e1)
+    }}}
+      Begin #prel
+    {{{ tphl, RET #tphl;
+        is_twophase_started tphl γ dinit objs_dom j K ls e1 e1 }}}.
+  Proof.
+    iIntros (Φ) "(?&Hatom) HΦ".
+    iNamed.
+    iNamed "Htwophase".
+    wp_apply (wp_TwoPhase__Begin_raw with "[$]"); first by assumption.
+    iIntros (?) "?".
+    iNamed.
+    iApply "HΦ".
+    iExists (∅, ∅), (∅, ∅), _.
+    iFrame.
+    iPureIntro.
+    split.
+    - apply always_steps_refl.
+      rewrite /wf_jrnl /offsets_aligned /sizes_correct dom_empty_L /=.
+      set_solver.
+    - rewrite /jrnl_maps_have_mt_changed /=.
+      split; first by reflexivity.
+      rewrite map_zip_empty_r.
+      apply map_Forall_empty.
+  Qed.
+
+  Theorem wp_TwoPhase__CommitNoRelease' l γ dinit objs_dom j K ls e1 v :
+    {{{ is_twophase_started l γ dinit objs_dom j K ls e1 (SOMEV v) }}}
       TwoPhase__CommitNoRelease #l
     {{{ (ok:bool), RET #ok;
         if ok then
-          is_twophase_releasable N l γ γ' dinit objs_dom ∗
+          is_twophase_releasable l γ objs_dom ∗
           j ⤇ K (SOMEV v)
         else
-          is_twophase_started N l γ γ' dinit objs_dom
-                              j K e1 (SOMEV v)
+          is_twophase_started l γ dinit objs_dom j K ls e1 (SOMEV v)
     }}}.
   Proof. Admitted.
 
-  Theorem twophase_started_abort N l γ γ' dinit objs_dom j K e1 e2 :
-    is_twophase_started N l γ γ' dinit objs_dom j K e1 e2 -∗
-    |NC={⊤}=> is_twophase_releasable N l γ γ' dinit objs_dom ∗
+  Theorem twophase_started_abort l γ dinit objs_dom j K ls e1 e2 :
+    is_twophase_started l γ dinit objs_dom j K ls e1 e2 -∗
+    |NC={⊤}=> is_twophase_releasable l γ objs_dom ∗
               j ⤇ K NONEV.
   Proof. Admitted.
 
-  Theorem wp_TwoPhase__ReleaseAll' N l γ γ' dinit objs_dom :
-    {{{ is_twophase_releasable N l γ γ' dinit objs_dom }}}
+  Theorem wp_TwoPhase__ReleaseAll' l γ objs_dom :
+    {{{ is_twophase_releasable l γ objs_dom }}}
       TwoPhase__ReleaseAll #l
     {{{ RET #(); True }}}.
   Proof. Admitted.
 
-  Theorem wp_TwoPhase__ReadBuf' N l γ γ' dinit objs_dom j K0 K
-          {Hctx: LanguageCtx' (ext := @spec_ext_op_field _)
-                              (ffi := (spec_ffi_model_field))
-                              (ffi_semantics := (spec_ext_semantics_field))
-                              K} e1 a sz :
-    {{{ is_twophase_started N l γ γ' dinit objs_dom j K0
-                            e1
-                            (K (ExternalOp (ext := @spec_ext_op_field jrnl_spec_ext)
-                                           ReadBufOp (PairV (addr2val' a) #sz))) }}}
+  Theorem wp_TwoPhase__ReadBuf' l γ dinit objs_dom j K0 K ls
+          {Hctx: LanguageCtx'
+            (ext := @spec_ext_op_field _)
+            (ffi := (spec_ffi_model_field))
+            (ffi_semantics := (spec_ext_semantics_field))
+            K} e1 a sz :
+    {{{
+      is_twophase_started l γ dinit objs_dom j K0 ls e1
+        (K (ExternalOp (ext := @spec_ext_op_field jrnl_spec_ext)
+          ReadBufOp (PairV (addr2val' a) #sz)))
+    }}}
       TwoPhase__ReadBuf' #l (addr2val a, #sz)
     {{{ v, RET (val_of_obj v);
-        is_twophase_started N l γ γ' dinit objs_dom j K0
-                            e1 (K (val_of_obj' v)) }}}.
+        is_twophase_started l γ dinit objs_dom j K0 ls e1
+          (K (val_of_obj' v))
+    }}}.
   Proof. Admitted.
 
-  Theorem wp_TwoPhase__OverWrite' N l γ γ' dinit objs_dom j K0 K
-          {Hctx: LanguageCtx' (ext := @spec_ext_op_field _)
-                                             (ffi := (spec_ffi_model_field))
-                                             (ffi_semantics := (spec_ext_semantics_field))
-                                             K}  e1 a ov :
-    {{{ is_twophase_started N l γ γ' dinit objs_dom j K0
-                            e1
-                            (K (ExternalOp (ext := @spec_ext_op_field jrnl_spec_ext)
-                                           OverWriteOp (PairV (addr2val' a) (val_of_obj' ov)))) }}}
+  Theorem wp_TwoPhase__OverWrite' l γ dinit objs_dom j K0 K ls
+          {Hctx: LanguageCtx'
+            (ext := @spec_ext_op_field _)
+            (ffi := (spec_ffi_model_field))
+            (ffi_semantics := (spec_ext_semantics_field))
+            K}  e1 a ov :
+    {{{
+      is_twophase_started l γ dinit objs_dom j K0 ls
+        e1
+        (K (ExternalOp (ext := @spec_ext_op_field jrnl_spec_ext)
+          OverWriteOp (PairV (addr2val' a) (val_of_obj' ov)))) }}}
       TwoPhase__OverWrite' #l (addr2val a, val_of_obj ov)
-    {{{  RET #();
-        is_twophase_started N l γ γ' dinit objs_dom j K0
-                            e1 (K #()) }}}.
+    {{{ RET #();
+        is_twophase_started l γ dinit objs_dom j K0 ls
+                            e1 (K #())
+    }}}.
   Proof. Admitted.
 
-  Lemma twophase_started_step_puredet N l γ γ' dinit objs_dom j K0 K
-        `{Hctx: LanguageCtx' (ext := @spec_ext_op_field _)
-                                             (ffi := (spec_ffi_model_field))
-                                             (ffi_semantics := (spec_ext_semantics_field))
-                                             K} e0 e1 e2:
+  Lemma twophase_started_step_puredet l γ dinit objs_dom j K0 K ls
+        `{Hctx: LanguageCtx'
+          (ext := @spec_ext_op_field _)
+          (ffi := (spec_ffi_model_field))
+          (ffi_semantics := (spec_ext_semantics_field))
+          K} e0 e1 e2:
     (∀ σ, prim_step' e1 σ [] e2 σ []) →
-    is_twophase_started N l γ γ' dinit objs_dom j K0 e0 (K e1) -∗
-    is_twophase_started N l γ γ' dinit objs_dom j K0 e0 (K e2).
+    is_twophase_started l γ dinit objs_dom j K0 ls e0 (K e1) -∗
+    is_twophase_started l γ dinit objs_dom j K0 ls e0 (K e2).
   Proof. Admitted.
 
-  Lemma twophase_started_ub_det N l γ γ' dinit objs_dom E j K0 K
-        `{Hctx: LanguageCtx' (ext := @spec_ext_op_field _)
-                                             (ffi := (spec_ffi_model_field))
-                                             (ffi_semantics := (spec_ext_semantics_field))
-                                             K} e0 e :
+  Lemma twophase_started_ub_det l γ dinit objs_dom E j K0 K ls
+        `{Hctx: LanguageCtx'
+          (ext := @spec_ext_op_field _)
+          (ffi := (spec_ffi_model_field))
+          (ffi_semantics := (spec_ext_semantics_field))
+          K} e0 e :
     nclose sN ⊆ E →
     (∀ s, stuck' e s) →
-    is_twophase_started N l γ γ' dinit objs_dom j K0 e0 (K e)
+    is_twophase_started l γ dinit objs_dom j K0 ls e0 (K e)
     -∗ |NC={E}=> False.
   Proof. Admitted.
 
