src/ShouldBuild.v
@@ -23,6 +23,7 @@ From Perennial.program_proof Require
      alloc_proof
      twophase.twophase_proof
      twophase.twophase_refinement_proof
+     (* twophase.wrapper_proof *)
      simple.proofs simple.example
      wp_to_wpc.
 From Perennial.program_proof.examples Require
